src/Star.v
@@ -1,0 +1,74 @@
+Set Implicit Arguments.
+
+(** STAR provides a type star to represent repeated applications of
+    an arbitrary binary relation R over values in A.
+
+    We will use star here to represent the transitive closure of an
+    action; that is, star a is an action where there is some sequence
+    m1 m2 ... mN where a m1 m2, a m2 m3, ... a mN-1 mN hold. *)
+Section STAR.
+
+  Variable A : Type.
+  Variable R : A -> A -> Prop.
+
+  Infix "-->" := R (at level 40).
+
+  Reserved Notation "s1 -->* s2" (at level 50).
+
+  Inductive star : A -> A -> Prop :=
+  | star_refl : forall s,
+    s -->* s
+  | star_step : forall s1 s2 s3,
+    s1 --> s2 ->
+    s2 -->* s3 ->
+    s1 -->* s3
+  where "s1 -->* s2" := (star s1 s2).
+
+  Hint Constructors star.
+
+  Reserved Notation "s1 ==>* s2" (at level 50).
+
+  Inductive star_r : A -> A -> Prop :=
+  | star_r_refl : forall s,
+    s ==>* s
+  | star_r_step : forall s1 s2 s3,
+    s1 ==>* s2 ->
+    s2 --> s3 ->
+    s1 ==>* s3
+  where "s2 ==>* s1" := (star_r s1 s2).
+
+  Hint Constructors star_r.
+
+  Lemma star_r_trans : forall s0 s1 s2,
+    s1 ==>* s2 ->
+    s0 ==>* s1 ->
+    s0 ==>* s2.
+  Proof.
+    induction 1; eauto.
+  Qed.
+
+  Hint Resolve star_r_trans.
+
+  Lemma star_trans : forall s0 s1 s2,
+    s0 -->* s1 ->
+    s1 -->* s2 ->
+    s0 -->* s2.
+  Proof.
+    induction 1; eauto.
+  Qed.
+
+  Hint Resolve star_trans.
+
+  Theorem star_lr_eq : forall s s',
+    s -->* s' <-> s ==>* s'.
+  Proof.
+    intros.
+    split; intros;
+      induction H; eauto.
+  Qed.
+
+
+End STAR.
+
+Hint Constructors star.
+Hint Constructors star_r.
